\subsection{Proofs}
\begin{enumerate}

    \item Give the terms of order $\leq 3$ in the power series:
    The trick for all of these is to just use their power series expansions or use ones we've found and stuff more $f$s into them 
    to get out more that one needs.
    \begin{enumerate}
      \item $e^z \sin(z)$
      \item $\sin z \cos z$
      \item $\frac{e^z - 1}{z}$
      \item $\frac{e^z - \cos z}{z}$
      \item $\frac{1}{\cos z}$
      \item $\frac{\cos z}{\sin z}$
      \item $\frac{\sin z}{\cos z}$
      \item $\frac{e^z}{\sin z}$
    \end{enumerate}
    
    \item Let $f(z) = \sum a_n z^n$.
  
    Define $f(-z) = \sum a_n (-z)^n = \sum a_n(-1)^n z^n$.
  
    Define $f$ as \textbf{even} if $a_n = 0$ for $n$ odd.
  
    Define $f$ as \textbf{odd} if $a_n = 0$ for $n$ even.
  
    Verify that $f$ is even if and only if $f(-z) = f(z)$ and $f$ is odd if and only if $f(-z) = -f(z).$
  
    \textbf{Proof}:
    Use power series expansions. Proving the \textbf{even} case first, but the same type of argument will work for the odd.
  
    If $f$ is \textbf{even} then $n$ is odd, so:
    \begin{align*}
      f(-z) &= \sum a_n z^n (-1)^n \\
      &= a_1 z (-1) + a_2 z^2 (-1)^2 + a_3 z^3 (-1)^3 \\
      &+ a_4 z^4 (-1)^4 + a_5 z^5 (-1)^5 + a_6 z^6 (-1)^6 + \cdots + a_n z^n (-1)^n \\
    \end{align*}
  
    Recall that since this is \textbf{even} then all the $a_n = 0$ for odd $n$ which leaves us 
    with (note $k \in \mathbb{N}$ here):
    \begin{align*}
      f(-z) &= a_2 z^2 (-1)^2 + a_4 z^4 (-1)^4 + a_6 z^6 (-1)^6 + \cdots + a_n z^{2k} (-1)^{2k} \\
    \end{align*} 
    Noticing that all of the factors of $(-1)$ have the form $(-1)^{2k}$ one sees:
    \begin{align*}
      f(-z) = f(z)
    \end{align*}
    Conversely, if you assume $f(-z) = f(z)$ then $f$ is \textbf{even} simply by definition, 
    which completes the proof for the \textbf{even} case. 
    
    A similar argument can be applied for the \textbf{odd} case.
    \qed
  
    \item Define the \textbf{Bernoulli numbers} $B_n$ by the power series:
  
    \begin{align*}
      \frac{z}{e^z - 1} = \sum_{n = 0}^{\infty}\frac{B_n}{n\,!}z^n \\
    \end{align*}
  
    Prove the recursion formula:
  
    \begin{align*}
      \frac{B_0}{n \, ! \; 0!} + \frac{B_1}{(n - 1)! \; 1!} + \cdots + \frac{B_{n - 1}}{1! \; (n - 1)\,!} + = 
      \begin{cases}
        1 \;\;\; \text{   if } n = 1. \\
        0 \;\;\; \text{   if } n > 1. \\
      \end{cases}
    \end{align*}
    Then $B_0 = 1.$
    
    Compute $B_1, B_2, B_3, B_4.$
    
    Show that $B_n = 0$ if $n$ is odd and $n \not = 1.$

    \textbf{Proof}:
    The given power series representation of the Bernoulli numbers is called the 
    generating function of Bernoulli numbers.

    To prove the recursion formula, you can use the power series differentiation rule of products
    which states that:

    \begin{align*}
      \frac{d}{dz}[f(z)g(z)] = f(z)\frac{dg(z)}{dz}+ g(z)\frac{df(z)}{dz} \\
    \end{align*}

    \begin{enumerate}

      \item Differentiate the equation with respect to $z$:
      \[\frac{1}{e^z - 1} - \frac{ze^z}{(e^z - 1)^2} = \sum_{n = 1}^{\infty}\frac{B_n}{(n-1)!}z^{n-1}\]

      \item Multiply the equation by $z^n$.
      
      \begin{align*}
        \frac{z^n}{e^z - 1} - \frac{z z^n}{(e^z - 1)^2}e^z &= \sum_{n = 1}^{\infty}\frac{B_n}{(n-1)!}z^{n-1} z^n \\
        \frac{z^n}{e^z - 1} - \frac{z^{n + 1} e^z}{(e^z - 1)^2} &= \sum_{n = 1}^{\infty}\frac{B_n}{(n-1)!}z^{2n-1} \\
      \end{align*}

      \item Integrate the equation with respect to $z$ from $0$ to $z$:
      \begin{align*}
        \int_{0}^{z} \left( \frac{z^n}{e^z - 1} - \frac{z^{n + 1} e^z}{(e^z - 1)^2} \right) dz &= \int_{0}^{z} \left( \sum_{n = 1}^{\infty}\frac{B_n}{(n-1)!}z^{2n-1} \right) dz \\
      \end{align*}

      \item Recall the $e^z$ power series representation:
    
      \[e^z = 1 + z + \frac{z^2}{2!} + \frac{z^3}{3!} + \cdots\]

      \item  Using this expansion and the assumption that the integral of a power series is the power series of the 
      integral, you can simplify the left side of the equation obtained in step (c) to:

      \begin{align*}
        \int_{0}^{z} \left( \frac{z^n}{e^z - 1} - \frac{z^{n + 1} e^z}{(e^z - 1)^2} \right) dz &= \int_{0}^{z} \left( \sum_{n = 1}^{\infty}\frac{B_n}{(n-1)!}z^{2n-1} \right) dz \\
      \end{align*}

      \item Now use the binomial formula:

      \begin{align*}
        (a + b)^n = \sum_{i = 0}^{n} {n \choose i} a^{n-i} b^i \\
      \end{align*}
      
      The property that the $B_n$ are defined 
      by the power series:
      \begin{align*}
        \frac{z}{e^z-1} = \sum_{n=0}^\infty \frac{B_n}{n!}z^n \\
      \end{align*}

      And:
      \begin{align*}
        \frac{d}{dz} e^z &= e^z \\
        \frac{d}{dz} z^n &= nz^{n-1} \\
      \end{align*}

      To tie this all together with those integrations and the binomials in the denominators possibly. 

    \end{enumerate}
    
    \item Show that:
  
    \begin{align*}
      \frac{z}{2} \frac{e^{z/2} + e^{-z/2}}{e^{z/2} - e^{-z/2}} = \sum_{n = 0}^\infty \frac{B_n}{(2n)!}z^{2n} \;. \\
    \end{align*}
  
    Replace $z$ by $2\pi i z$ to show that:
  
    \begin{align*}
      \pi z \cot(\pi z) = \sum_{n = 0}^\infty (-1)^n \frac{(2\pi)^{2n}}{(2n)!} z^{2n} B_{2n} \;.
    \end{align*}
  
    \item Express the power series for $\tan z , \frac{z}{\sin z}, z \cot z ,$ in terms of \textbf{Bernoulli numbers}.
  
    \item (\textbf{Difference Equation}) given complex numbers $a_0, a_1, u_1, u_2 \;$ define $a_n$ for $2 \leq n$ by:
  
    \begin{align*}
      a_n = u_1 a_{n - 1} +u_2 a_{n - 2} \;.
    \end{align*}
  
    If you have a factorization: \textbf{STOPPED}
  \end{enumerate}
  \newpage